\documentclass[11pt]{article}
\usepackage{style}
\title{Differential Equations Week \textbf{7}}
\author{Garud Shah}
\begin{document}
    \maketitle \newpage 
    \begin{problem}[Problem 1, generalized]
        \setcounter{equation}{-1}
        Find extra particular solutions to the differential equation 
        \begin{align}
            y'' - 2xy' + \lambda y = 0.
        \end{align}
        for $\lambda=4,6$.
    \end{problem}
    \begin{solution}
        Consider $4x^{\lambda/2}$. We get, plugging in to the differential operator:
        \begin{align}
            \lambda\left(\lambda - 2\right)x^{\lambda/2 - 2}.
        \end{align}
        For $\lambda = 4$, this gives the constant $8$ needed whixh means we just need to subtract two, giving $2x^2-1$ asour first solution. \\
        At $6$, we get $24x$, and try $kx$ to subtract $6x$ giving $2x^3 - 3x$ for this equation. \\
        Reduction of order time! For $\lambda = 4,6$ in top, bottom respectivly: (use eqn. 8 in the textbook)
        \begin{align}
            \boxed{(2x^2 - 1) \int \dfrac{e^{x^2}}{(2x^2-1)^2}dx} \\
            \boxed{(3x^2 - 2x) \int \dfrac{e^{x^2}}{(3x^2-2x)^2}dx} \\
        \end{align}  
    \end{solution}
    \newpage
    \begin{problem}[Problem 2]
        Solve the differential equation 
        \begin{align}
            (x^2-1)y'' -2xy' + 2y = 0.
        \end{align}
    \end{problem}
    \begin{solution}
        Immediately try $xf$. We get:
        \begin{align}
            (x^2-1)(f' + xf'') - 2x(f+f'x) + 2fx &= 0 \\
            x^2f' - f' + x^3f'' - xf'' - 2fx + 2f'x^2 + 2fx &= 0 \\
            (x^3-x)f'' + 3f'(x^2-1) &= 0 \\
            3f' &= xf'' \\
            f' &= x^3 \\
            f &\equiv x^4 \\
            y(x) &= c_1x+c_2x^4.
        \end{align}
    \end{solution}
\end{document}