\documentclass[11pt]{article}
\usepackage{gstyle}
\title{Differential Equations Week \textbf{12}}
\author{Garud Shah}
\begin{document}
    \maketitle \newpage 
    \begin{problem}
        Solve the following differential equation:
        \begin{align}
            \begin{cases}
                P' &= P(c-r(N)) \\
                Q' &= Pr(N) \\
                N &= P+Q
            \end{cases}
        \end{align}
        for 
        \begin{enumerate}[(a)]
            \item $r(N) = b(1+\log N)$, $P(0)=1$, $Q(0)=0$, $N(0)=1$
            \item $r(N) = (2N-1)s$. 
        \end{enumerate}
    \end{problem}
    \begin{solution}
        Note that $Q(t)$ is very annoying, let's turn this into an $P, N$ differential equation system.
        \begin{align}
            &\begin{cases}
                P' &= P(c-r(N)) \\
                N' &= cP 
            \end{cases}.
        \end{align}
        Now we solve the phase plane differential equation,
        \begin{align}
            \dfrac{dP}{dN} &= \dfrac{c-r(N)}{c} \\
            P &= N - \dfrac{1}{c} \int_{dontcare}^N\ r(x) \, dx +\alpha.
        \end{align}
        Now, plug back in:
        \begin{align}
            N' &= c\left(\displaystyle N - \dfrac{1}{c} \int_{dontcare}^N\ r(x) \, dx  +\alpha\right) \\
            t &= \int \dfrac{1}{cN - \int_{dontcare}^N\ r(x) \, dx  +c\alpha} \, dN 
        \end{align}
    \end{solution}\newpage
    \begin{solution}
        Plug in (set dontcare to 1):
        \begin{align}
            t &= \int \dfrac{1}{cN - b N\log N} \, dN  \\
            &= \int \dfrac{1}{N} \cdot \dfrac{1}{c-b \log N} \, dN \\
            &= \int \dfrac{1}{c-bu} \, du \\
            &= -\dfrac{1}{b}\log | c-b\log|N||+C \\
            c-ae^{-bt} &= b \log|N| \\\
            N &= e^{\frac{1}{b}(c-ae^{-bt})} \\
            P &= e^{\frac{1}{b}(c-ae^{-bt})} - \dfrac{1}{c} N\log N \\
            &= e^{\frac{1}{b}(c-ae^{-bt})}\left(1-\frac{1}{bc}(c-ae^{-bt})\right)
        \end{align}
    \end{solution}
    \begin{solution}
        Plug in (set dontcare to 0):
        \begin{align}
            t &= \int \dfrac{1}{cN - sN + sN^2} \, dN \\
            &= \int \dfrac{1}{N(c-s+sN)} \, dN \\
            &= \dfrac{1}{s} \int \dfrac{1}{N(N-1+c/s)} \, dN \\
            &= \dfrac{1}{c-s}\log \left|\dfrac{N}{N-1+c/s} \right| \\
            e^{t(c-s)} &= \dfrac{N}{N-1+c/s} \\
            N(1-e^{t(c-s)}) 
        \end{align}
    \end{solution}
\end{document}